Update blob basefee link and simulate to v103

RocqOfRust/revm/revm_interpreter/instructions/simulate/block_info/blob_basefee.v
@@ -1,22 +1,16 @@
 Require Import simulate.RocqOfRust.
 Require Import alloy_primitives.links.aliases.
-Require Import core.simulate.default.
-Require Import core.simulate.option.
 Require Import revm.revm_context_interface.links.host.
-Require Import revm.revm_context_interface.simulate.block.
 Require Import revm.revm_context_interface.simulate.host.
-Require Import revm.revm_interpreter.gas.simulate.constants.
 Require Import revm.revm_interpreter.instructions.links.block_info.
 Require Import revm.revm_interpreter.instructions.simulate.macros.
-Require Import revm.revm_interpreter.links.gas.
+Require Import revm.revm_interpreter.links.instruction_context.
 Require Import revm.revm_interpreter.links.interpreter.
 Require Import revm.revm_interpreter.links.interpreter_types.
-Require Import revm.revm_interpreter.simulate.gas.
 Require Import revm.revm_interpreter.simulate.interpreter_types.
 Require Import revm.revm_primitives.links.hardfork.
 Require Import revm.revm_primitives.simulate.hardfork.
 Require Import ruint.links.lib.
-Require Import ruint.simulate.from.
 
 Definition blob_basefee
     {WIRE H : Set} `{Link WIRE} `{Link H}
@@ -28,16 +22,11 @@ Definition blob_basefee
     (host : H) :
     Interpreter.t WIRE WIRE_types * H :=
   check_macro interpreter SpecId.CANCUN (fun interpreter => (interpreter, host)) (fun interpreter =>
-  gas_macro interpreter constants.BASE (fun interpreter => (interpreter, host)) (fun interpreter =>
-  let block :=
-    IHost.(Host.BlockGetter_for_Self).(BlockGetter.block).(RefStub.projection) host in
-  let price :=
-    Impl_Option.unwrap_or_default
-      (IHost.(Host.BlockGetter_for_Self).(BlockGetter.Block_for_Block).(Block.blob_gasprice) block) in
-  push_macro interpreter {| Uint.value := i[price] |}
+  let '(price, host) := IHost.(Host.blob_gasprice) host in
+  push_macro interpreter price
     (fun interpreter => (interpreter, host)) (fun interpreter =>
   (interpreter, host)
-  ))).
+  )).
 
 Lemma blob_basefee_eq
     {WIRE H : Set} `{Link WIRE} `{Link H}
@@ -54,9 +43,13 @@ Lemma blob_basefee_eq
     (host : H) :
   let ref_interpreter : '&mut (Interpreter.t WIRE WIRE_types) := make_ref 0 in
   let ref_host : '&mut H := make_ref 1 in
+  let context := {|
+    instruction_context.InstructionContext.interpreter := ref_interpreter;
+    instruction_context.InstructionContext.host := ref_host;
+  |} in
   {{
     SimulateM.eval_f
-      (run_blob_basefee run_InterpreterTypes_for_WIRE run_Host_for_H ref_interpreter ref_host)
+      (run_blob_basefee run_InterpreterTypes_for_WIRE run_Host_for_H context)
       ([interpreter; host]%stack) 🌲
     (
       Output.Success tt,
@@ -68,19 +61,16 @@ Proof.
   intros.
   with_strategy transparent [run_blob_basefee] unfold blob_basefee, run_blob_basefee; cbn.
   check_macro_eq InterpreterTypesEq.
-  gas_macro_eq idtac.
-  s. {
-    apply HostEq.
+  destruct (IHost.(Host.blob_gasprice) host) as [price host'] eqn:?; cbn.
+  apply Run.LetUnfold.
+  eapply Run.Call.
+  {
+    s. {
+      eapply (Host.Eq.blob_gasprice (t := HostEq)).
+    }
+    s.
   }
-  s. {
-    s_apply HostEq.
-  }
-  s. {
-    apply Impl_Option.unwrap_or_default_eq.
-  }
-  s. {
-    s_apply Impl_Uint.from_eq.
-  }
+  rewrite Heqp; cbn.
   push_macro_eq InterpreterTypesEq.
-  s.
+  { s. }
 Qed.
