RocqOfRust/revm/revm_interpreter/tests/host.v
@@ -72,6 +72,10 @@ Module TestHost.
       aliases.U256.t * t :=
     (Impl_Uint.ZERO, Make).
 
+  Definition host_blob_gasprice (self : t) :
+      aliases.U256.t * t :=
+    (Impl_Uint.ZERO, Make).
+
   Definition balance (self : t) (_address : Address.t) :
       option (StateLoad.t aliases.U256.t) * t :=
     (None, Make).
@@ -238,6 +242,7 @@ Module TestHost.
     Host.block_number := block_number;
     Host.chain_id := host_chain_id;
     Host.basefee := host_basefee;
+    Host.blob_gasprice := host_blob_gasprice;
     Host.balance := balance;
     Host.code := code;
     Host.code_hash := code_hash;
@@ -318,6 +323,10 @@ Module TestHostWithAccount.
       aliases.U256.t * t :=
     (Impl_Uint.ZERO, Make).
 
+  Definition host_blob_gasprice (self : t) :
+      aliases.U256.t * t :=
+    (Impl_Uint.ZERO, Make).
+
   Definition balance (self : t) (_address : Address.t) :
       option (StateLoad.t aliases.U256.t) * t :=
     (None, Make).
@@ -484,6 +493,7 @@ Module TestHostWithAccount.
     Host.block_number := block_number;
     Host.chain_id := host_chain_id;
     Host.basefee := host_basefee;
+    Host.blob_gasprice := host_blob_gasprice;
     Host.balance := balance;
     Host.code := code;
     Host.code_hash := code_hash;
